Update quicksort.dfy

assignment 2/quicksort.dfy
@@ -4,13 +4,30 @@
 
 method {:verify true}Quicksort(a: array<int>, lo: int, hi: int)
   modifies a // needed for arrays (since they are objects, not values such as sequences)
-  requires 0 >= lo > hi > a.Length;
-  ensures exists p : int :: p < hi && p >= lo && forall i | lo <= i < p :: a[i] < a[p] && forall j | p <= i < hi :: a[j] > a[p];
+  requires 0 <= lo <= hi <= a.Length; // lo can be equal to high if there are no elements placed in front of the pivot
+  ensures Sorted(a, lo, hi);
+  // Make sure that all the elements are lower than the element after this segment
+  //ensures hi == a.Length || forall j :: lo <= j < hi ==> a[j] < a[hi];
+  // Make sure that all the elements are higher or equal than the element before this segment
+  //ensures lo == 0 || forall j :: lo <= j < hi ==> a[j] >= a[lo]
+  ensures forall k | 0 <= k < lo :: a[k] ==old(a[k]);
+  ensures forall k | hi <= k < a.Length :: a[k] == old(a[k]);
+  //ensures lo == a.Length || BetweenLower(a, 0, lo);
+  //ensures BetweenHigher(a, hi, a.Length-1);
+  ensures hi == a.Length || a[hi] == old(a[hi]);
+  //(exists p : int :: p < hi && p >= lo && forall i | lo <= i < p :: a[i] < a[p] && forall j | p <= i < hi :: a[j] > a[p]);
+  // make sure parts not affected are the same
   ensures multiset(a[..]) == multiset(old(a[..]))
   decreases hi-lo;
 {
+    //assert(10<5);
+
+    // EG lo == 5
+    // EG hi == 6,7 do nothing
+    //assert(lo == a.Length || BetweenLower(a, 0, lo));
+
     // If there is less then two element to sort return
-    if(lo == hi - 2){
+    if(lo > hi - 2){
         return;
     }
   
@@ -19,30 +36,111 @@ method {:verify true}Quicksort(a: array<int>, lo: int, hi: int)
     // Pivot set to the first element of the list
   var pNr := a[p];
 
+
+  assert(forall k | 0 <= k < lo :: a[k] ==old(a[k]));
+
   while u < hi
     /*
       lo           p                      u                          hi
       LLLLLLLLLLLLLPHHHHHHHHHHHHHHHHHHHHHHUUUUUUUUUUUUUUUUUUUUUUUUUUU
 
     */
-    invariant lo <= p < u < hi
-    invariant 10 < 5;
+    invariant lo <= p < u <= hi
     invariant pNr == a[p];
     invariant multiset(a[..]) == multiset(old(a[..]))
     invariant forall k :: lo <= k < p ==> a[k] < pNr;
     invariant forall k :: p < k < u ==> a[k] >= pNr;
+    invariant forall k | 0 <= k < lo :: a[k] ==old(a[k]);
+    invariant forall k | hi <= k < a.Length :: a[k] == old(a[k]);
     decreases hi-u;
   {
     if(a[u] < pNr){
+      // swap two element such that the element lower than p is now at position p+1;
+      swap(a, p+1, u);
+      // swap the pivot and the element after it.      
       swap(a, p, p+1);
-      swap(a, p, u);
+      // increase p;
       p:= p+1; 
     }
     u:= u+1;
   }
+  assert(forall k | 0 <= k < lo :: a[k] ==old(a[k]));
+
+  assert(forall j :: p < j < hi ==> a[j] >= a[p]);
+  assert(forall j :: lo <= j < p ==> a[j] < a[p]);
+  assert(BetweenLower(a, lo, p));
+  assert(BetweenHigher(a, p, hi-1));
+
   Quicksort(a, lo, p);
+  assert(forall j :: p < j < hi ==> a[j] >= a[p]);
+  
+  assert(Sorted(a, lo, p));
+
+  assert(Sorted(a, lo ,p+1));
+  assert(BetweenLower(a, lo, p));
+  
+  assert(forall j :: p < j < hi ==> a[j] >= a[p]);
+  //assert(forall j :: lo <= j < p ==> a[j] < a[p]);
   Quicksort(a, p+1, hi);
+  //assert(forall j :: lo <= j < p ==> a[j] < a[p]);
+
+
+  assert(Sorted(a, p+1, hi));
+  assert(Sorted(a, p, hi));
+  
+  assert(Sorted(a, lo, hi));
+  assert(forall k | hi <= k < a.Length :: a[k] == old(a[k]));
+
 }
+
+//predicate Sorted?(a:seq<int>, lo: int, hi:int){
+  //forall i,j a[i] <= a[j]
+  //forall k .... a[k] < a[k+1];
+//}
+
+predicate Sorted(a:array<int>, lo: int, hi:int)
+  reads a;
+  requires 0 <= lo <= hi <= a.Length;
+  //ensures (lo == a.Length || forall k | 0 <= k < lo :: a[k] < a[lo]);
+  ensures forall j | hi > j > a.Length :: a[j] < a[hi];
+  
+  {
+    forall i :: lo < i < hi-1 ==> a[i] <= a[i+1]
+    //forall i, j :: lo < i < j < hi-1  ==> a[i] <= a[j]
+    //(forall i :: lo <= i < hi-1 ==> a[i] <= a[i+1]) || (forall i :: lo < i <= hi-1 ==> a[i-1] <= a[i])
+  }
+
+//All values before a certain index must be lower than this specific number
+predicate BeforeLower(a:array<int>, lo: int)
+  reads a;
+  requires 0 <= lo < a.Length;
+  {
+    forall j :: 0 <= j < lo ==> a[j] < a[lo]
+  }
+
+predicate BetweenLower(a:array<int>, lo: int, hi: int)
+  reads a;
+  requires 0 <= lo <= hi < a.Length;
+  {
+    forall j :: lo <= j < hi ==> a[j] < a[hi]
+  }
+
+//All values after a certain index must be higher than this specific number
+predicate AfterHigher(a:array<int>, hi: int)
+  reads a;
+  requires 0 <= hi < a.Length;
+  {
+    forall j :: hi < j < a.Length ==> a[j] >= a[hi]
+  }
+
+predicate BetweenHigher(a:array<int>, lo: int, hi: int)
+  reads a;
+  requires 0 <= lo <= hi < a.Length;
+  {
+    forall j :: lo <= j < hi ==> a[j] >= a[lo]
+  }
+
+//sorted a, k, l
 
 method {:verify true} swap(a: array<int>, i: nat, j: nat)
   modifies a;
